completed atomic case of lemma 2

gentzen.v
@@ -413,6 +413,14 @@ match (correctness a) with
 end.
 
 
+(* Axioms of PA_omega *)
+(* *)
+Definition pa_omega_axiom (a : formula) : bool :=
+match a with
+| atom a' => correct_a a'
+| _ => false
+end.
+
 
 (* Basic properties of lists and lists of nats *)
 (* *)
@@ -567,40 +575,40 @@ Fixpoint closed_term_list (a : formula) : list term :=
    variable x_n in a formula f *)
 (* *)
 Fixpoint substitution_t (f : term) (n : nat) (t : term) : term :=
-  match f with
-    zero => f
-  | succ f_1 => succ (substitution_t f_1 n t)
-  | plus f_1 f_2 => plus (substitution_t f_1 n t) (substitution_t f_2 n t)
-  | times f_1 f_2 => times (substitution_t f_1 n t) (substitution_t f_2 n t)
-  | f_var m =>
-      (match (beq_nat m n) with
-        true => t
-      | false => f
-      end)
-  | b_var m =>
-      (match (beq_nat m n) with
-        true => t
-      | false => f
-      end)
-  end.
+match f with
+| zero => f
+| succ f_1 => succ (substitution_t f_1 n t)
+| plus f_1 f_2 => plus (substitution_t f_1 n t) (substitution_t f_2 n t)
+| times f_1 f_2 => times (substitution_t f_1 n t) (substitution_t f_2 n t)
+| f_var m =>
+    (match (beq_nat m n) with
+    | true => t
+    | false => f
+    end)
+| b_var m =>
+    (match (beq_nat m n) with
+    | true => t
+    | false => f
+    end)
+end.
 
 Definition substitution_a (f : atomic_formula) (n : nat) (t : term)
   : atomic_formula :=
-  match f with
-    equ t_1 t_2 => equ (substitution_t t_1 n t) (substitution_t t_2 n t)
-  end.
+match f with
+  equ t_1 t_2 => equ (substitution_t t_1 n t) (substitution_t t_2 n t)
+end.
 
 Fixpoint substitution (f : formula) (n : nat) (t : term) : formula :=
-  match f with
-    atom a => atom (substitution_a a n t)
-  | neg f_1 => neg (substitution f_1 n t)
-  | lor f_1 f_2 => lor (substitution f_1 n t) (substitution f_2 n t)
-  | univ m f_1 => 
-      (match (beq_nat m n) with
-        true => f
-      | false => univ m (substitution f_1 n t)
-      end)
-  end.
+match f with
+| atom a => atom (substitution_a a n t)
+| neg f_1 => neg (substitution f_1 n t)
+| lor f_1 f_2 => lor (substitution f_1 n t) (substitution f_2 n t)
+| univ m f_1 => 
+    (match (beq_nat m n) with
+    | true => f
+    | false => univ m (substitution f_1 n t)
+    end)
+end.
 
 (* Given a list of closed terms and a variable x_n in formula a, check if any
 of those terms can be substituted for x_n to obtain the formula b *)
@@ -628,18 +636,126 @@ in a formula f; namely, that no free occurrence of x_n in f is in the scope of
 some (univ m), where x_m is a variable in t. *)
 (* *)
 Fixpoint free_for (t : term) (n : nat) (f : formula) : bool :=
-  match f with
-    atom a => true
-  | neg f_1 => free_for t n f_1
-  | lor f_1 f_2 => (free_for t n f_1) && (free_for t n f_2)
-  | univ m f_1 =>
-      if member m (free_list_t t)
-      then negb (member n (free_list f_1))
-      else free_for t n f_1
-  end.
+match f with
+| atom a => true
+| neg f_1 => free_for t n f_1
+| lor f_1 f_2 => (free_for t n f_1) && (free_for t n f_2)
+| univ m f_1 =>
+    if member m (free_list_t t)
+    then negb (member n (free_list f_1))
+    else free_for t n f_1
+end.
 
 Compute free_for zero 0 (univ 1 (atom (equ (b_var 0) (b_var 0)))).
 Compute free_for (b_var 1) 0 (univ 1 (atom (equ (b_var 0) (b_var 0)))).
+
+
+(* Lemma 2 *)
+(* *)
+Lemma stuff : forall (T s : term) (n : nat),
+  eval T > 0 -> eval (substitution_t T n s) > 0.
+Proof.
+intros.
+induction T.
+- auto.
+- case_eq (eval T); intros.
+  + inversion H.
+Admitted.
+
+
+
+Lemma x : forall (T s t : term) (n : nat),
+  eval s = eval t -> eval (substitution_t T n s) = eval (substitution_t T n t).
+Proof.
+intros.
+induction T.
+- auto.
+- assert (substitution_t (succ T) n s = succ (substitution_t T n s)). { auto. }
+  assert (substitution_t (succ T) n t = succ (substitution_t T n t)). { auto. }
+  rewrite H0. rewrite H1. case_eq (eval (substitution_t T n s));
+  intros; simpl; rewrite <- IHT; rewrite H2; auto.
+- assert (eval (substitution_t (plus T1 T2) n s) =
+          eval (plus (substitution_t T1 n s) (substitution_t T2 n s))). { auto. }
+  assert (eval (substitution_t (plus T1 T2) n t) =
+          eval (plus (substitution_t T1 n t) (substitution_t T2 n t))). { auto. }
+  rewrite H0. rewrite H1. case_eq (eval (substitution_t T1 n s));
+  intros; simpl; rewrite <- IHT1; rewrite <- IHT2; rewrite H2; auto.
+- assert (eval (substitution_t (times T1 T2) n s) =
+          eval (times (substitution_t T1 n s) (substitution_t T2 n s))). { auto. }
+  assert (eval (substitution_t (times T1 T2) n t) =
+          eval (times (substitution_t T1 n t) (substitution_t T2 n t))). { auto. }
+  rewrite H0. rewrite H1. case_eq (eval (substitution_t T1 n s));
+  intros; simpl; rewrite <- IHT1; rewrite <- IHT2; rewrite H2; auto.
+- simpl. case (beq_nat n0 n). apply H. auto.
+- simpl. case (beq_nat n0 n). apply H. auto.
+Qed.
+
+Lemma x1 : forall (a : atomic_formula) (s t : term) (n : nat),
+  eval s = eval t ->
+  correctness (substitution_a a n s) = correct ->
+  correctness (substitution_a a n t) = correct.
+Proof.
+intros.
+case_eq a.
+intros t1 t2 H1.
+rewrite H1 in H0.
+unfold substitution_a in H0.
+unfold substitution_a.
+pose proof (x t1 s t n H) as Ht1.
+pose proof (x t2 s t n H) as Ht2.
+case_eq (eval (substitution_t t1 n t));
+case_eq (eval (substitution_t t2 n t)); intros;
+unfold correctness in H0;
+rewrite Ht1 in H0; rewrite Ht2 in H0;
+rewrite H2 in H0; rewrite H3 in H0; inversion H0.
+simpl. rewrite H2. rewrite H3. auto.
+Qed.
+
+
+Lemma x2 : forall (s t : term),
+  correct_a (equ s t) = true -> eval s = eval t.
+Proof.
+intros s t.
+unfold correct_a.
+unfold correctness.
+case_eq (eval s); case_eq (eval t); intros.
+- auto.
+- inversion H1.
+- inversion H1.
+- case_eq (beq_nat (S n0) (S n)).
+  + apply nat_eq_beq.
+  + intros. rewrite H2 in H1. inversion H1.
+Qed.
+
+
+
+Theorem lemma_2_atomic : forall (s t : term) (a : atomic_formula) (n : nat),
+  correct_a (equ s t) = true ->
+  pa_omega_axiom (substitution (atom a) n s) = true ->
+  pa_omega_axiom (substitution (atom a) n t) = true.
+Proof.
+simpl. intros.
+assert (eval s = eval t). { apply x2. apply H. }
+assert (correctness (substitution_a a n s) = correct).
+{ inversion H0. unfold correct_a in H3.
+  case_eq (correctness (substitution_a a n s)); intros;
+  rewrite H2 in H3; inversion H3; auto. }
+pose proof (x1 a s t n H1 H2).
+unfold correct_a.
+rewrite H3. auto.
+Qed.
+
+
+
+
+
+
+
+
+
+
+
+
 
 
 (* Logical axioms of FOL *)
